<?xml version="1.0"?>
<rdf:RDF xmlns="http://ontologies.sparna.fr/sparnatural-config-datasources#"
     xml:base="http://ontologies.sparna.fr/sparnatural-config-datasources"
     xmlns:owl="http://www.w3.org/2002/07/owl#"
     xmlns:rdf="http://www.w3.org/1999/02/22-rdf-syntax-ns#"
     xmlns:xml="http://www.w3.org/XML/1998/namespace"
     xmlns:xsd="http://www.w3.org/2001/XMLSchema#"
     xmlns:rdfs="http://www.w3.org/2000/01/rdf-schema#"
     xmlns:sparnatural-config-core="http://data.sparna.fr/ontologies/sparnatural-config-core#"
     xmlns:sparnatural-config-datasources="http://data.sparna.fr/ontologies/sparnatural-config-datasources#">
    <owl:Ontology rdf:about="http://data.sparna.fr/ontologies/sparnatural-config-datasources">
        <owl:imports rdf:resource="http://data.sparna.fr/ontologies/sparnatural-config-core"/>
    </owl:Ontology>
    


    <!-- 
    ///////////////////////////////////////////////////////////////////////////////////////
    //
    // Annotation properties
    //
    ///////////////////////////////////////////////////////////////////////////////////////
     -->

    


    <!-- http://data.sparna.fr/ontologies/sparnatural-config-datasources#childrenPath -->

    <owl:AnnotationProperty rdf:about="http://data.sparna.fr/ontologies/sparnatural-config-datasources#childrenPath">
        <rdfs:comment xml:lang="en">The SPARQL property path where the children of resources can be read. This must be a valid SPARQL property path without any prefix, e.g. &lt;http://schema.org&gt; (including brackets).</rdfs:comment>
        <rdfs:label xml:lang="en">children path</rdfs:label>
    </owl:AnnotationProperty>
    


    <!-- http://data.sparna.fr/ontologies/sparnatural-config-datasources#childrenProperty -->

    <owl:AnnotationProperty rdf:about="http://data.sparna.fr/ontologies/sparnatural-config-datasources#childrenProperty">
        <rdfs:comment xml:lang="en">The URI of a property where the children of resources can be read. This should point to a URI.</rdfs:comment>
        <rdfs:label xml:lang="en">children property</rdfs:label>
    </owl:AnnotationProperty>
    


    <!-- http://data.sparna.fr/ontologies/sparnatural-config-datasources#datasource -->

    <owl:AnnotationProperty rdf:about="http://data.sparna.fr/ontologies/sparnatural-config-datasources#datasource">
        <rdfs:comment xml:lang="en">The datasource from which a property with value selection should fetch its data.</rdfs:comment>
        <rdfs:label xml:lang="en">datasource</rdfs:label>
        <rdfs:range rdf:resource="http://data.sparna.fr/ontologies/sparnatural-config-datasources#Datasource"/>
    </owl:AnnotationProperty>
    


    <!-- http://data.sparna.fr/ontologies/sparnatural-config-datasources#labelPath -->

    <owl:AnnotationProperty rdf:about="http://data.sparna.fr/ontologies/sparnatural-config-datasources#labelPath">
        <rdfs:comment xml:lang="en">The SPARQL property path where the label of resources can be read. This must be a valid SPARQL property path without any prefix, e.g. &lt;http://schema.org&gt; (including brackets).</rdfs:comment>
        <rdfs:label xml:lang="en">label path</rdfs:label>
        <rdfs:range rdf:resource="http://www.w3.org/2001/XMLSchema#string"/>
        <rdfs:domain rdf:resource="http://data.sparna.fr/ontologies/sparnatural-config-datasources#SparqlDatasource"/>
    </owl:AnnotationProperty>
    


    <!-- http://data.sparna.fr/ontologies/sparnatural-config-datasources#labelProperty -->

    <owl:AnnotationProperty rdf:about="http://data.sparna.fr/ontologies/sparnatural-config-datasources#labelProperty">
        <rdfs:comment xml:lang="en">The URI of a property where the label of resources can be read. This should point to a URI.</rdfs:comment>
        <rdfs:label xml:lang="en">label property</rdfs:label>
        <rdfs:domain rdf:resource="http://data.sparna.fr/ontologies/sparnatural-config-datasources#SparqlDatasource"/>
    </owl:AnnotationProperty>
    


    <!-- http://data.sparna.fr/ontologies/sparnatural-config-datasources#noSort -->

    <owl:AnnotationProperty rdf:about="http://data.sparna.fr/ontologies/sparnatural-config-datasources#noSort">
        <rdfs:comment xml:lang="en">Set this to true to disable client-side javascript sorting for a datasource. If set to true, the order of elements will be the one returned by the SPARQL query.</rdfs:comment>
        <rdfs:label xml:lang="en">no sort</rdfs:label>
        <rdfs:range rdf:resource="http://www.w3.org/2001/XMLSchema#boolean"/>
        <rdfs:domain rdf:resource="http://data.sparna.fr/ontologies/sparnatural-config-datasources#SparqlDatasource"/>
    </owl:AnnotationProperty>
    


    <!-- http://data.sparna.fr/ontologies/sparnatural-config-datasources#treeChildrenDatasource -->

    <owl:AnnotationProperty rdf:about="http://data.sparna.fr/ontologies/sparnatural-config-datasources#treeChildrenDatasource">
        <rdfs:comment xml:lang="en">A reference to the datasource with which a tree widget will populate the children of a node in the tree.</rdfs:comment>
        <rdfs:label xml:lang="en">tree children datasource</rdfs:label>
        <rdfs:subPropertyOf rdf:resource="http://data.sparna.fr/ontologies/sparnatural-config-datasources#datasource"/>
    </owl:AnnotationProperty>
    


    <!-- http://data.sparna.fr/ontologies/sparnatural-config-datasources#treeRootsDatasource -->

    <owl:AnnotationProperty rdf:about="http://data.sparna.fr/ontologies/sparnatural-config-datasources#treeRootsDatasource">
        <rdfs:comment xml:lang="en">A reference to the datasource with which a tree widget will populate its root (first-level) nodes.</rdfs:comment>
        <rdfs:label xml:lang="en">tree roots datasource</rdfs:label>
        <rdfs:subPropertyOf rdf:resource="http://data.sparna.fr/ontologies/sparnatural-config-datasources#datasource"/>
    </owl:AnnotationProperty>
    


    <!-- 
    ///////////////////////////////////////////////////////////////////////////////////////
    //
    // Object Properties
    //
    ///////////////////////////////////////////////////////////////////////////////////////
     -->

    


    <!-- http://data.sparna.fr/ontologies/sparnatural-config-datasources#queryTemplate -->

    <owl:ObjectProperty rdf:about="http://data.sparna.fr/ontologies/sparnatural-config-datasources#queryTemplate">
        <rdfs:domain rdf:resource="http://data.sparna.fr/ontologies/sparnatural-config-datasources#SparqlDatasource"/>
        <rdfs:range rdf:resource="http://data.sparna.fr/ontologies/sparnatural-config-datasources#SPARQLQuery"/>
        <rdfs:comment xml:lang="en">The SPARQL query template to be used in a SPARQL datasource.

The SPARQL template holds a SPARQL query string in which the placeholders $domain, $property, $range will be replaced by their corresponding values before executing the query.

For autocomplete field, the additionnal placeholders $key and $lang will also be replaced by their corresponding values before executing the query

The placeholder $labelPath will be replaced by the value indicated in the SparqlDatasource in the labelPath (for a full SPARQL property path) or labelProperty (for a single property URI).</rdfs:comment>
        <rdfs:label xml:lang="en">query template</rdfs:label>
    </owl:ObjectProperty>
    


    <!-- 
    ///////////////////////////////////////////////////////////////////////////////////////
    //
    // Data properties
    //
    ///////////////////////////////////////////////////////////////////////////////////////
     -->

    


    <!-- http://data.sparna.fr/ontologies/sparnatural-config-datasources#queryString -->

    <owl:DatatypeProperty rdf:about="http://data.sparna.fr/ontologies/sparnatural-config-datasources#queryString">
        <rdfs:domain>
            <owl:Class>
                <owl:unionOf rdf:parseType="Collection">
                    <rdf:Description rdf:about="http://data.sparna.fr/ontologies/sparnatural-config-datasources#SPARQLQuery"/>
                    <rdf:Description rdf:about="http://data.sparna.fr/ontologies/sparnatural-config-datasources#SparqlDatasource"/>
                </owl:unionOf>
            </owl:Class>
        </rdfs:domain>
        <rdfs:range rdf:resource="http://www.w3.org/2001/XMLSchema#string"/>
        <rdfs:comment xml:lang="en">The query string of a SPARQLQuery, or directly on a SPARQLDatasource</rdfs:comment>
        <rdfs:label xml:lang="en">query string</rdfs:label>
    </owl:DatatypeProperty>
    


    <!-- http://data.sparna.fr/ontologies/sparnatural-config-datasources#sparqlEndpointUrl -->

    <owl:DatatypeProperty rdf:about="http://data.sparna.fr/ontologies/sparnatural-config-datasources#sparqlEndpointUrl">
        <rdfs:domain rdf:resource="http://data.sparna.fr/ontologies/sparnatural-config-datasources#SparqlDatasource"/>
        <rdfs:range rdf:resource="http://www.w3.org/2001/XMLSchema#anyURI"/>
        <rdfs:comment xml:lang="en">A SPARQL endpoint URL to which the query should be sent.</rdfs:comment>
        <rdfs:label xml:lang="en">SPARQL endpoint URL</rdfs:label>
    </owl:DatatypeProperty>
    


    <!-- 
    ///////////////////////////////////////////////////////////////////////////////////////
    //
    // Classes
    //
    ///////////////////////////////////////////////////////////////////////////////////////
     -->

    


    <!-- http://data.sparna.fr/ontologies/sparnatural-config-datasources#Datasource -->

    <owl:Class rdf:about="http://data.sparna.fr/ontologies/sparnatural-config-datasources#Datasource">
        <rdfs:comment xml:lang="en">A source of data to populate Sparnatural widgets (list, search fields, trees, etc.)</rdfs:comment>
        <rdfs:label xml:lang="en">Datasource</rdfs:label>
    </owl:Class>
    


    <!-- http://data.sparna.fr/ontologies/sparnatural-config-datasources#SPARQLQuery -->

    <owl:Class rdf:about="http://data.sparna.fr/ontologies/sparnatural-config-datasources#SPARQLQuery">
        <rdfs:comment xml:lang="en">A SPARQL query, holding its query string</rdfs:comment>
        <rdfs:label xml:lang="en">SPARQL Query</rdfs:label>
    </owl:Class>
    


    <!-- http://data.sparna.fr/ontologies/sparnatural-config-datasources#SparqlDatasource -->

    <owl:Class rdf:about="http://data.sparna.fr/ontologies/sparnatural-config-datasources#SparqlDatasource">
        <rdfs:subClassOf rdf:resource="http://data.sparna.fr/ontologies/sparnatural-config-datasources#Datasource"/>
        <rdfs:comment xml:lang="en">A source of data for a Sparnatural widget implemented as a SPARQL query.</rdfs:comment>
        <rdfs:label xml:lang="en">SPARQL datasource</rdfs:label>
    </owl:Class>
    


    <!-- http://data.sparna.fr/ontologies/sparnatural-config-datasources#SparqlListDatasource -->

    <owl:Class rdf:about="http://data.sparna.fr/ontologies/sparnatural-config-datasources#SparqlListDatasource">
        <rdfs:subClassOf rdf:resource="http://data.sparna.fr/ontologies/sparnatural-config-datasources#SparqlDatasource"/>
        <rdfs:comment xml:lang="en">A datasource to populate a list widget, implemented as a SPARQL query.

The SPARQL query MUST return 2 variables : ?label and either ?uri or ?value (if returning a literal). It can return other variables as well.

The following variables, if present in the SPARQL query, are automatically bound in the query :
  - $domain: bound to the URI of the subject class of the criteria
  - $property: bound to the URI or property path of the property of the criteria
  - $range: bound to the URI of the object class of the criteria
  - $lang: bound to the default language of Sparnatural
  - $type: bound to the typePredicate parameter of Sparnatural, rdf:type by default</rdfs:comment>
        <rdfs:label xml:lang="en">SPARQL list datasource</rdfs:label>
    </owl:Class>
    


    <!-- http://data.sparna.fr/ontologies/sparnatural-config-datasources#SparqlSearchDatasource -->

    <owl:Class rdf:about="http://data.sparna.fr/ontologies/sparnatural-config-datasources#SparqlSearchDatasource">
        <rdfs:subClassOf rdf:resource="http://data.sparna.fr/ontologies/sparnatural-config-datasources#SparqlDatasource"/>
        <rdfs:comment xml:lang="en">A datasource to populate an autocomplete search widget, implemented as a SPARQL query.

The SPARQL query MUST return 2 variables : ?label and either ?uri or ?value (if returning a literal). It can return other variables as well;

The following variables, if present in the SPARQL query, are automatically bound in the query :
  - $domain: bound to the URI of the subject class of the criteria
  - $property: bound to the URI or property path of the property of the criteria
  - $range: bound to the URI of the object class of the criteria
  - $lang: bound to the default language of Sparnatural
  - $key: the characters entered by the user in the search field
  - $type: bound to the typePredicate parameter of Sparnatural, rdf:type by default</rdfs:comment>
        <rdfs:label xml:lang="en">SPARQL search datasource</rdfs:label>
    </owl:Class>
    


    <!-- http://data.sparna.fr/ontologies/sparnatural-config-datasources#SparqlTreeChildrenDatasource -->

    <owl:Class rdf:about="http://data.sparna.fr/ontologies/sparnatural-config-datasources#SparqlTreeChildrenDatasource">
        <rdfs:subClassOf rdf:resource="http://data.sparna.fr/ontologies/sparnatural-config-datasources#SparqlDatasource"/>
        <rdfs:comment xml:lang="en">A datasource to populate the children of a node of a tree widget, when unfolded, implemented as a SPARQL query.

The query MUST return the following variables:
  - ?uri
  - ?label
  - ?hasChildren: a boolean indicating if the node has some children

In addition the query CAN return the following variables:
  - ?count: the number of times this entity is used as the value of the criteria</rdfs:comment>
        <rdfs:label xml:lang="en">SPARQL tree datasource for children of a node</rdfs:label>
    </owl:Class>
    


    <!-- http://data.sparna.fr/ontologies/sparnatural-config-datasources#SparqlTreeRootDatasource -->

    <owl:Class rdf:about="http://data.sparna.fr/ontologies/sparnatural-config-datasources#SparqlTreeRootDatasource">
        <rdfs:subClassOf rdf:resource="http://data.sparna.fr/ontologies/sparnatural-config-datasources#SparqlDatasource"/>
        <rdfs:comment xml:lang="en">A datasource to populate the root of a tree widget, implemented as a SPARQL query.</rdfs:comment>
        <rdfs:label xml:lang="en">SPARQL tree datasource for the roots of the tree</rdfs:label>
    </owl:Class>
    


    <!-- 
    ///////////////////////////////////////////////////////////////////////////////////////
    //
    // Individuals
    //
    ///////////////////////////////////////////////////////////////////////////////////////
     -->

    


    <!-- http://data.sparna.fr/ontologies/sparnatural-config-datasources#list_URI_alpha -->

    <owl:NamedIndividual rdf:about="http://data.sparna.fr/ontologies/sparnatural-config-datasources#list_URI_alpha">
        <rdf:type rdf:resource="http://data.sparna.fr/ontologies/sparnatural-config-datasources#SparqlListDatasource"/>
        <sparnatural-config-datasources:queryTemplate rdf:resource="http://data.sparna.fr/ontologies/sparnatural-config-datasources#query_list_URI_alpha"/>
        <rdfs:comment xml:lang="en">A datasource that returns a list of entities with their URI as a label ordered alphabetically based on the URI string.</rdfs:comment>
    </owl:NamedIndividual>
    


    <!-- http://data.sparna.fr/ontologies/sparnatural-config-datasources#list_URI_count -->

    <owl:NamedIndividual rdf:about="http://data.sparna.fr/ontologies/sparnatural-config-datasources#list_URI_count">
        <rdf:type rdf:resource="http://data.sparna.fr/ontologies/sparnatural-config-datasources#SparqlListDatasource"/>
        <sparnatural-config-datasources:queryTemplate rdf:resource="http://data.sparna.fr/ontologies/sparnatural-config-datasources#query_list_URI_count"/>
        <sparnatural-config-datasources:noSort rdf:datatype="http://www.w3.org/2001/XMLSchema#boolean">true</sparnatural-config-datasources:noSort>
        <rdfs:comment xml:lang="en">A datasource that returns a list of entities with their URI as a label ordered by the descending number of times the entity is used as a value.

This is typically the default behavior for a list without a datasource specified.</rdfs:comment>
    </owl:NamedIndividual>
    


    <!-- http://data.sparna.fr/ontologies/sparnatural-config-datasources#list_URI_or_literal_alpha -->

    <owl:NamedIndividual rdf:about="http://data.sparna.fr/ontologies/sparnatural-config-datasources#list_URI_or_literal_alpha">
        <rdf:type rdf:resource="http://data.sparna.fr/ontologies/sparnatural-config-datasources#SparqlListDatasource"/>
        <sparnatural-config-datasources:queryTemplate rdf:resource="http://data.sparna.fr/ontologies/sparnatural-config-datasources#query_list_URI_or_literal_alpha"/>
        <rdfs:comment xml:lang="en">A datasource that returns a list of URI or Literals, ordered alphabetically based on their string representation. It can work indifferently with URIs or Literal values.</rdfs:comment>
    </owl:NamedIndividual>
    


    <!-- http://data.sparna.fr/ontologies/sparnatural-config-datasources#list_URI_or_literal_alpha_with_count -->

    <owl:NamedIndividual rdf:about="http://data.sparna.fr/ontologies/sparnatural-config-datasources#list_URI_or_literal_alpha_with_count">
        <rdf:type rdf:resource="http://data.sparna.fr/ontologies/sparnatural-config-datasources#SparqlListDatasource"/>
        <sparnatural-config-datasources:queryTemplate rdf:resource="http://data.sparna.fr/ontologies/sparnatural-config-datasources#query_list_URI_or_literal_alpha_with_count"/>
        <rdfs:comment xml:lang="en">A datasource that returns a list of URIs or Literals, ordered alphabetically based on their string representation, with their number of occurrences in parenthesis.</rdfs:comment>
    </owl:NamedIndividual>
    


    <!-- http://data.sparna.fr/ontologies/sparnatural-config-datasources#list_URI_or_literal_count -->

    <owl:NamedIndividual rdf:about="http://data.sparna.fr/ontologies/sparnatural-config-datasources#list_URI_or_literal_count">
        <rdf:type rdf:resource="http://data.sparna.fr/ontologies/sparnatural-config-datasources#SparqlListDatasource"/>
        <sparnatural-config-datasources:queryTemplate rdf:resource="http://data.sparna.fr/ontologies/sparnatural-config-datasources#query_list_URI_or_literal_count"/>
        <rdfs:comment xml:lang="en">A datasource that returns a list of URI or Literals, ordered on their descending number of occurrences. It can work indifferently with URIs or Literal values.</rdfs:comment>
    </owl:NamedIndividual>
    


    <!-- http://data.sparna.fr/ontologies/sparnatural-config-datasources#list_dctermstitle_alpha -->

    <owl:NamedIndividual rdf:about="http://data.sparna.fr/ontologies/sparnatural-config-datasources#list_dctermstitle_alpha">
        <rdf:type rdf:resource="http://data.sparna.fr/ontologies/sparnatural-config-datasources#SparqlListDatasource"/>
        <sparnatural-config-datasources:queryTemplate rdf:resource="http://data.sparna.fr/ontologies/sparnatural-config-datasources#query_list_label_alpha"/>
        <sparnatural-config-datasources:labelProperty rdf:resource="http://purl.org/dc/terms/title"/>
        <rdfs:comment xml:lang="en">A datasource that returns a list of entities with their dcterms:title ordered alphabetically based on this property.</rdfs:comment>
    </owl:NamedIndividual>
    


    <!-- http://data.sparna.fr/ontologies/sparnatural-config-datasources#list_dctermstitle_alpha_with_count -->

    <owl:NamedIndividual rdf:about="http://data.sparna.fr/ontologies/sparnatural-config-datasources#list_dctermstitle_alpha_with_count">
        <rdf:type rdf:resource="http://data.sparna.fr/ontologies/sparnatural-config-datasources#SparqlListDatasource"/>
        <sparnatural-config-datasources:queryTemplate rdf:resource="http://data.sparna.fr/ontologies/sparnatural-config-datasources#query_list_label_alpha_with_count"/>
        <rdfs:comment xml:lang="en">A datasource that returns a list of entities with their dcterms:title and the number of occurrences of the entity in parenthesis, ordered alphabetically based on this property.</rdfs:comment>
    </owl:NamedIndividual>
    


    <!-- http://data.sparna.fr/ontologies/sparnatural-config-datasources#list_dctermstitle_count -->

    <owl:NamedIndividual rdf:about="http://data.sparna.fr/ontologies/sparnatural-config-datasources#list_dctermstitle_count">
        <rdf:type rdf:resource="http://data.sparna.fr/ontologies/sparnatural-config-datasources#SparqlListDatasource"/>
        <sparnatural-config-datasources:queryTemplate rdf:resource="http://data.sparna.fr/ontologies/sparnatural-config-datasources#query_list_label_count"/>
        <sparnatural-config-datasources:labelProperty rdf:resource="http://purl.org/dc/terms/title"/>
        <sparnatural-config-datasources:noSort rdf:datatype="http://www.w3.org/2001/XMLSchema#boolean">true</sparnatural-config-datasources:noSort>
        <rdfs:comment xml:lang="en">A datasource that returns a list of entities with their dcterms:title ordered by the descending number of times the entity is used as a value.</rdfs:comment>
    </owl:NamedIndividual>
    


    <!-- http://data.sparna.fr/ontologies/sparnatural-config-datasources#list_foafname_alpha -->

    <owl:NamedIndividual rdf:about="http://data.sparna.fr/ontologies/sparnatural-config-datasources#list_foafname_alpha">
        <rdf:type rdf:resource="http://data.sparna.fr/ontologies/sparnatural-config-datasources#SparqlListDatasource"/>
        <sparnatural-config-datasources:queryTemplate rdf:resource="http://data.sparna.fr/ontologies/sparnatural-config-datasources#query_list_label_alpha"/>
        <sparnatural-config-datasources:labelProperty rdf:resource="http://xmlns.com/foaf/0.1/name"/>
        <rdfs:comment xml:lang="en">A datasource that returns a list of entities with their foaf:name ordered alphabetically based on this property.</rdfs:comment>
    </owl:NamedIndividual>
    


    <!-- http://data.sparna.fr/ontologies/sparnatural-config-datasources#list_foafname_alpha_with_count -->

    <owl:NamedIndividual rdf:about="http://data.sparna.fr/ontologies/sparnatural-config-datasources#list_foafname_alpha_with_count">
        <rdf:type rdf:resource="http://data.sparna.fr/ontologies/sparnatural-config-datasources#SparqlListDatasource"/>
        <sparnatural-config-datasources:queryTemplate rdf:resource="http://data.sparna.fr/ontologies/sparnatural-config-datasources#query_list_label_alpha_with_count"/>
        <sparnatural-config-datasources:labelProperty rdf:resource="http://xmlns.com/foaf/0.1/name"/>
        <rdfs:comment xml:lang="en">A datasource that returns a list of entities with their foaf:name and the number of occurrences of the entity in parenthesis, ordered alphabetically based on this property.</rdfs:comment>
    </owl:NamedIndividual>
    


    <!-- http://data.sparna.fr/ontologies/sparnatural-config-datasources#list_foafname_count -->

    <owl:NamedIndividual rdf:about="http://data.sparna.fr/ontologies/sparnatural-config-datasources#list_foafname_count">
        <rdf:type rdf:resource="http://data.sparna.fr/ontologies/sparnatural-config-datasources#SparqlListDatasource"/>
        <sparnatural-config-datasources:queryTemplate rdf:resource="http://data.sparna.fr/ontologies/sparnatural-config-datasources#query_list_label_count"/>
        <sparnatural-config-datasources:labelProperty rdf:resource="http://xmlns.com/foaf/0.1/name"/>
        <sparnatural-config-datasources:noSort rdf:datatype="http://www.w3.org/2001/XMLSchema#boolean">true</sparnatural-config-datasources:noSort>
        <rdfs:comment xml:lang="en">A datasource that returns a list of entities with their foaf:name ordered by the descending number of times the entity is used as a value.</rdfs:comment>
    </owl:NamedIndividual>
    


    <!-- http://data.sparna.fr/ontologies/sparnatural-config-datasources#list_rdfslabel_alpha -->

    <owl:NamedIndividual rdf:about="http://data.sparna.fr/ontologies/sparnatural-config-datasources#list_rdfslabel_alpha">
        <rdf:type rdf:resource="http://data.sparna.fr/ontologies/sparnatural-config-datasources#SparqlListDatasource"/>
        <sparnatural-config-datasources:queryTemplate rdf:resource="http://data.sparna.fr/ontologies/sparnatural-config-datasources#query_list_label_alpha"/>
        <sparnatural-config-datasources:labelProperty rdf:resource="http://www.w3.org/2000/01/rdf-schema#label"/>
        <rdfs:comment xml:lang="en">A datasource that returns a list of entities with their rdfs:label ordered alphabetically based on this property.</rdfs:comment>
    </owl:NamedIndividual>
    


    <!-- http://data.sparna.fr/ontologies/sparnatural-config-datasources#list_rdfslabel_alpha_with_count -->

    <owl:NamedIndividual rdf:about="http://data.sparna.fr/ontologies/sparnatural-config-datasources#list_rdfslabel_alpha_with_count">
        <rdf:type rdf:resource="http://data.sparna.fr/ontologies/sparnatural-config-datasources#SparqlListDatasource"/>
        <sparnatural-config-datasources:queryTemplate rdf:resource="http://data.sparna.fr/ontologies/sparnatural-config-datasources#query_list_label_alpha_with_count"/>
        <sparnatural-config-datasources:labelProperty rdf:resource="http://www.w3.org/2000/01/rdf-schema#label"/>
        <rdfs:comment xml:lang="en">A datasource that returns a list of entities with their rdfs:label and the number of occurrences of the entity in parenthesis, ordered alphabetically based on this property.</rdfs:comment>
    </owl:NamedIndividual>
    


    <!-- http://data.sparna.fr/ontologies/sparnatural-config-datasources#list_rdfslabel_count -->

    <owl:NamedIndividual rdf:about="http://data.sparna.fr/ontologies/sparnatural-config-datasources#list_rdfslabel_count">
        <rdf:type rdf:resource="http://data.sparna.fr/ontologies/sparnatural-config-datasources#SparqlListDatasource"/>
        <sparnatural-config-datasources:queryTemplate rdf:resource="http://data.sparna.fr/ontologies/sparnatural-config-datasources#query_list_label_count"/>
        <sparnatural-config-datasources:labelProperty rdf:resource="http://www.w3.org/2000/01/rdf-schema#label"/>
        <sparnatural-config-datasources:noSort rdf:datatype="http://www.w3.org/2001/XMLSchema#boolean">true</sparnatural-config-datasources:noSort>
        <rdfs:comment xml:lang="en">A datasource that returns a list of entities with their rdfs:label ordered by the descending number of times the entity is used as a value.</rdfs:comment>
    </owl:NamedIndividual>
    


    <!-- http://data.sparna.fr/ontologies/sparnatural-config-datasources#list_schemaname_alpha -->

    <owl:NamedIndividual rdf:about="http://data.sparna.fr/ontologies/sparnatural-config-datasources#list_schemaname_alpha">
        <rdf:type rdf:resource="http://data.sparna.fr/ontologies/sparnatural-config-datasources#SparqlListDatasource"/>
        <sparnatural-config-datasources:queryTemplate rdf:resource="http://data.sparna.fr/ontologies/sparnatural-config-datasources#query_list_label_alpha"/>
        <sparnatural-config-datasources:labelProperty rdf:resource="http://schema.org/name"/>
        <rdfs:comment xml:lang="en">A datasource that returns a list of entities with their schema:name ordered alphabetically based on this property.</rdfs:comment>
    </owl:NamedIndividual>
    


    <!-- http://data.sparna.fr/ontologies/sparnatural-config-datasources#list_schemaname_alpha_with_count -->

    <owl:NamedIndividual rdf:about="http://data.sparna.fr/ontologies/sparnatural-config-datasources#list_schemaname_alpha_with_count">
        <rdf:type rdf:resource="http://data.sparna.fr/ontologies/sparnatural-config-datasources#SparqlListDatasource"/>
        <sparnatural-config-datasources:queryTemplate rdf:resource="http://data.sparna.fr/ontologies/sparnatural-config-datasources#query_list_label_alpha_with_count"/>
        <rdfs:comment xml:lang="en">A datasource that returns a list of entities with their schema:name and the number of occurrences of the entity in parenthesis, ordered alphabetically based on this property.</rdfs:comment>
    </owl:NamedIndividual>
    


    <!-- http://data.sparna.fr/ontologies/sparnatural-config-datasources#list_schemaname_count -->

    <owl:NamedIndividual rdf:about="http://data.sparna.fr/ontologies/sparnatural-config-datasources#list_schemaname_count">
        <rdf:type rdf:resource="http://data.sparna.fr/ontologies/sparnatural-config-datasources#SparqlListDatasource"/>
        <sparnatural-config-datasources:queryTemplate rdf:resource="http://data.sparna.fr/ontologies/sparnatural-config-datasources#query_list_label_count"/>
        <sparnatural-config-datasources:labelProperty rdf:resource="http://schema.org/name"/>
        <sparnatural-config-datasources:noSort rdf:datatype="http://www.w3.org/2001/XMLSchema#boolean">true</sparnatural-config-datasources:noSort>
        <rdfs:comment xml:lang="en">A datasource that returns a list of entities with their schema:name ordered by the descending number of times the entity is used as a value.</rdfs:comment>
    </owl:NamedIndividual>
    


    <!-- http://data.sparna.fr/ontologies/sparnatural-config-datasources#list_skospreflabel_alpha -->

    <owl:NamedIndividual rdf:about="http://data.sparna.fr/ontologies/sparnatural-config-datasources#list_skospreflabel_alpha">
        <rdf:type rdf:resource="http://data.sparna.fr/ontologies/sparnatural-config-datasources#SparqlListDatasource"/>
        <sparnatural-config-datasources:queryTemplate rdf:resource="http://data.sparna.fr/ontologies/sparnatural-config-datasources#query_list_label_alpha"/>
        <sparnatural-config-datasources:labelProperty rdf:resource="http://www.w3.org/2004/02/skos/core#prefLabel"/>
        <rdfs:comment xml:lang="en">A datasource that returns a list of entities with their skos:prefLabel ordered alphabetically based on this property.</rdfs:comment>
    </owl:NamedIndividual>
    


    <!-- http://data.sparna.fr/ontologies/sparnatural-config-datasources#list_skospreflabel_alpha_with_count -->

    <owl:NamedIndividual rdf:about="http://data.sparna.fr/ontologies/sparnatural-config-datasources#list_skospreflabel_alpha_with_count">
        <rdf:type rdf:resource="http://data.sparna.fr/ontologies/sparnatural-config-datasources#SparqlListDatasource"/>
        <sparnatural-config-datasources:queryTemplate rdf:resource="http://data.sparna.fr/ontologies/sparnatural-config-datasources#query_list_label_alpha_with_count"/>
        <sparnatural-config-datasources:labelProperty rdf:resource="http://www.w3.org/2004/02/skos/core#prefLabel"/>
        <rdfs:comment xml:lang="en">A datasource that returns a list of entities with their skos:prefLabel and the number of occurrences of the entity in parenthesis, ordered alphabetically based on this property.</rdfs:comment>
    </owl:NamedIndividual>
    


    <!-- http://data.sparna.fr/ontologies/sparnatural-config-datasources#list_skospreflabel_count -->

    <owl:NamedIndividual rdf:about="http://data.sparna.fr/ontologies/sparnatural-config-datasources#list_skospreflabel_count">
        <rdf:type rdf:resource="http://data.sparna.fr/ontologies/sparnatural-config-datasources#SparqlListDatasource"/>
        <sparnatural-config-datasources:queryTemplate rdf:resource="http://data.sparna.fr/ontologies/sparnatural-config-datasources#query_list_label_count"/>
        <sparnatural-config-datasources:labelProperty rdf:resource="http://www.w3.org/2004/02/skos/core#prefLabel"/>
        <sparnatural-config-datasources:noSort rdf:datatype="http://www.w3.org/2001/XMLSchema#boolean">true</sparnatural-config-datasources:noSort>
        <rdfs:comment xml:lang="en">A datasource that returns a list of entities with their skos:prefLabel ordered by the descending number of times the entity is used as a value.</rdfs:comment>
    </owl:NamedIndividual>
    


    <!-- http://data.sparna.fr/ontologies/sparnatural-config-datasources#literal_list_alpha -->

    <owl:NamedIndividual rdf:about="http://data.sparna.fr/ontologies/sparnatural-config-datasources#literal_list_alpha">
        <rdf:type rdf:resource="http://data.sparna.fr/ontologies/sparnatural-config-datasources#SparqlListDatasource"/>
        <sparnatural-config-datasources:queryTemplate rdf:resource="http://data.sparna.fr/ontologies/sparnatural-config-datasources#query_literal_list_alpha"/>
        <rdfs:comment xml:lang="en">A datasource that returns a list of literal ordered alphabetically.</rdfs:comment>
    </owl:NamedIndividual>
    


    <!-- http://data.sparna.fr/ontologies/sparnatural-config-datasources#literal_list_alpha_with_count -->

    <owl:NamedIndividual rdf:about="http://data.sparna.fr/ontologies/sparnatural-config-datasources#literal_list_alpha_with_count">
        <rdf:type rdf:resource="http://data.sparna.fr/ontologies/sparnatural-config-datasources#SparqlListDatasource"/>
        <sparnatural-config-datasources:queryTemplate rdf:resource="http://data.sparna.fr/ontologies/sparnatural-config-datasources#query_literal_list_alpha_with_count"/>
        <rdfs:comment xml:lang="en">A datasource that returns a list of literal with count in parenthesis, ordered alphabetically.</rdfs:comment>
    </owl:NamedIndividual>
    


    <!-- http://data.sparna.fr/ontologies/sparnatural-config-datasources#literal_list_count -->

    <owl:NamedIndividual rdf:about="http://data.sparna.fr/ontologies/sparnatural-config-datasources#literal_list_count">
        <rdf:type rdf:resource="http://data.sparna.fr/ontologies/sparnatural-config-datasources#SparqlListDatasource"/>
        <sparnatural-config-datasources:queryTemplate rdf:resource="http://data.sparna.fr/ontologies/sparnatural-config-datasources#query_literal_list_count"/>
        <sparnatural-config-datasources:noSort rdf:datatype="http://www.w3.org/2001/XMLSchema#boolean">true</sparnatural-config-datasources:noSort>
        <rdfs:comment xml:lang="en">A datasource that returns a list of literal ordered by descending number of occurrences.</rdfs:comment>
    </owl:NamedIndividual>
    


    <!-- http://data.sparna.fr/ontologies/sparnatural-config-datasources#query_list_URI_alpha -->

    <owl:NamedIndividual rdf:about="http://data.sparna.fr/ontologies/sparnatural-config-datasources#query_list_URI_alpha">
        <rdf:type rdf:resource="http://data.sparna.fr/ontologies/sparnatural-config-datasources#SPARQLQuery"/>
        <sparnatural-config-datasources:queryString>SELECT DISTINCT ?uri (STR(?uri) AS ?label)
WHERE {
    ?domain $type $domain .
    ?domain $property ?uri .
    FILTER(isIRI(?uri))
    # Note how the range criteria is not used in this query
}
ORDER BY UCASE(STR(?label))
LIMIT 500</sparnatural-config-datasources:queryString>
    </owl:NamedIndividual>
    


    <!-- http://data.sparna.fr/ontologies/sparnatural-config-datasources#query_list_URI_count -->

    <owl:NamedIndividual rdf:about="http://data.sparna.fr/ontologies/sparnatural-config-datasources#query_list_URI_count">
        <rdf:type rdf:resource="http://data.sparna.fr/ontologies/sparnatural-config-datasources#SPARQLQuery"/>
        <sparnatural-config-datasources:queryString>SELECT ?uri ?count (CONCAT(STR(?uri), &apos; (&apos;, STR(?count), &apos;)&apos;) AS ?label) (STR(?uri) AS ?itemLabel)
WHERE {
{
  SELECT DISTINCT ?uri (COUNT(?domain) AS ?count)
  WHERE {
    ?domain $type $domain .
    ?domain $property ?uri .
    FILTER(isIRI(?uri))
    # Note how the range criteria is not used in this query
  }
  GROUP BY ?uri
}
}
ORDER BY DESC(?count) UCASE(STR(?label))
LIMIT 500</sparnatural-config-datasources:queryString>
    </owl:NamedIndividual>
    


    <!-- http://data.sparna.fr/ontologies/sparnatural-config-datasources#query_list_URI_or_literal_alpha -->

    <owl:NamedIndividual rdf:about="http://data.sparna.fr/ontologies/sparnatural-config-datasources#query_list_URI_or_literal_alpha">
        <rdf:type rdf:resource="http://data.sparna.fr/ontologies/sparnatural-config-datasources#SPARQLQuery"/>
        <sparnatural-config-datasources:queryString>SELECT DISTINCT ?value (CONCAT(IF(isLiteral(?value) &amp;&amp; LANG(?value) != &apos;&apos; &amp;&amp; LANG(?value) != $lang,CONCAT(STR(?value), &quot; &lt;sup&gt;(&quot;,LANG(?value),&quot;)&lt;/sup&gt;&quot;),STR(?value))) AS ?label)
WHERE {
    ?domain $type $domain .
    {
      {
        ?domain $property ?value . FILTER(isIRI(?value))
      }
      UNION
      {
        ?domain $property ?value . 
        FILTER(isLiteral(?value) &amp;&amp; (lang(?value) = $lang))
      }
      UNION
      {
        ?domain $property ?value . 
        FILTER(isLiteral(?value) &amp;&amp; (lang(?value) = $defaultLang))
        FILTER NOT EXISTS {
          ?domain $property ?valuePrefLang .
          FILTER(LANG(?valuePrefLang) = $lang)
        }
      }
      UNION
      {
        ?domain $property ?value . 
        FILTER(isLiteral(?value) &amp;&amp; (lang(?value) = &quot;&quot;))
        FILTER NOT EXISTS {
          ?domain $property ?valueAnyLang .
          FILTER((LANG(?valueAnyLang) = $lang) || (LANG(?valueAnyLang) = $defaultLang))
        }
      }
    }
    # Note how the range criteria is not used in this query
}
ORDER BY UCASE(STR(?label))
LIMIT 500</sparnatural-config-datasources:queryString>
    </owl:NamedIndividual>
    


    <!-- http://data.sparna.fr/ontologies/sparnatural-config-datasources#query_list_URI_or_literal_alpha_with_count -->

    <owl:NamedIndividual rdf:about="http://data.sparna.fr/ontologies/sparnatural-config-datasources#query_list_URI_or_literal_alpha_with_count">
        <rdf:type rdf:resource="http://data.sparna.fr/ontologies/sparnatural-config-datasources#SPARQLQuery"/>
        <sparnatural-config-datasources:queryString>SELECT DISTINCT ?value ?count (CONCAT(IF(isLiteral(?value) &amp;&amp; LANG(?value) != &apos;&apos; &amp;&amp; LANG(?value) != $lang,CONCAT(STR(?value), &quot; &lt;sup&gt;(&quot;,LANG(?value),&quot;)&lt;/sup&gt;&quot;),STR(?value)), &apos; (&apos;, STR(?count), &apos;)&apos;) AS ?label) (STR(?value) AS ?itemLabel)
WHERE {
{
  SELECT DISTINCT ?value (COUNT(DISTINCT ?domain) AS ?count)
  WHERE {
    ?domain $type $domain .
    {
      {
        ?domain $property ?value . FILTER(isIRI(?value))
      }
      UNION
      {
        ?domain $property ?value . 
        FILTER(isLiteral(?value) &amp;&amp; (lang(?value) = $lang))
      }
      UNION
      {
        ?domain $property ?value . 
        FILTER(isLiteral(?value) &amp;&amp; (lang(?value) = $defaultLang))
        FILTER NOT EXISTS {
          ?domain $property ?valuePrefLang .
          FILTER(LANG(?valuePrefLang) = $lang)
        }
      }
      UNION
      {
        ?domain $property ?value . 
        FILTER(isLiteral(?value) &amp;&amp; (lang(?value) = &quot;&quot;))
        FILTER NOT EXISTS {
          ?domain $property ?valueAnyLang .
          FILTER((LANG(?valueAnyLang) = $lang) || (LANG(?valueAnyLang) = $defaultLang))
        }
      }      
    }
  }
  GROUP BY ?value
}
}
ORDER BY UCASE(STR(?label))
LIMIT 500</sparnatural-config-datasources:queryString>
    </owl:NamedIndividual>
    


    <!-- http://data.sparna.fr/ontologies/sparnatural-config-datasources#query_list_URI_or_literal_count -->

    <owl:NamedIndividual rdf:about="http://data.sparna.fr/ontologies/sparnatural-config-datasources#query_list_URI_or_literal_count">
        <rdf:type rdf:resource="http://data.sparna.fr/ontologies/sparnatural-config-datasources#SPARQLQuery"/>
        <sparnatural-config-datasources:queryString>SELECT ?value ?count (CONCAT(IF(isLiteral(?value) &amp;&amp; LANG(?value) != &apos;&apos; &amp;&amp; LANG(?value) != $lang,CONCAT(STR(?value), &quot; &lt;sup&gt;(&quot;,LANG(?value),&quot;)&lt;/sup&gt;&quot;),STR(?value)), &apos; (&apos;, STR(?count), &apos;)&apos;) AS ?label) (STR(?value) AS ?itemLabel)
WHERE {
{
  SELECT DISTINCT ?value (COUNT(DISTINCT ?domain) AS ?count)
  WHERE {
    ?domain $type $domain .
    {
      {
        ?domain $property ?value . FILTER(isIRI(?value))
      }
      UNION
      {
        ?domain $property ?value . 
        FILTER(isLiteral(?value) &amp;&amp; (lang(?value) = $lang))
      }
      UNION
      {
        ?domain $property ?value . 
        FILTER(isLiteral(?value) &amp;&amp; (lang(?value) = $defaultLang))
        FILTER NOT EXISTS {
          ?domain $property ?valuePrefLang .
          FILTER(LANG(?valuePrefLang) = $lang)
        }
      }
      UNION
      {
        ?domain $property ?value . 
        FILTER(isLiteral(?value) &amp;&amp; (lang(?value) = &quot;&quot;))
        FILTER NOT EXISTS {
          ?domain $property ?valueAnyLang .
          FILTER((LANG(?valueAnyLang) = $lang) || (LANG(?valueAnyLang) = $defaultLang))
        }
      }      
    }
  }
  GROUP BY ?value
}
}
ORDER BY DESC(?count) UCASE(STR(?label))
LIMIT 500</sparnatural-config-datasources:queryString>
        <sparnatural-config-datasources:noSort rdf:datatype="http://www.w3.org/2001/XMLSchema#boolean">true</sparnatural-config-datasources:noSort>
    </owl:NamedIndividual>
    


    <!-- http://data.sparna.fr/ontologies/sparnatural-config-datasources#query_list_label_alpha -->

    <owl:NamedIndividual rdf:about="http://data.sparna.fr/ontologies/sparnatural-config-datasources#query_list_label_alpha">
        <rdf:type rdf:resource="http://data.sparna.fr/ontologies/sparnatural-config-datasources#SPARQLQuery"/>
        <sparnatural-config-datasources:queryString>SELECT DISTINCT ?uri ?label
WHERE {
    ?domain $type $domain .
    ?domain $property ?uri .
    # Note how the range criteria is not used in this query
    ?uri $labelPath ?label .
    FILTER(isIRI(?uri))
    FILTER(lang(?label) = &quot;&quot; || lang(?label) = $lang)
}
ORDER BY UCASE(STR(?label))
LIMIT 500</sparnatural-config-datasources:queryString>
    </owl:NamedIndividual>
    


    <!-- http://data.sparna.fr/ontologies/sparnatural-config-datasources#query_list_label_alpha_with_count -->

    <owl:NamedIndividual rdf:about="http://data.sparna.fr/ontologies/sparnatural-config-datasources#query_list_label_alpha_with_count">
        <rdf:type rdf:resource="http://data.sparna.fr/ontologies/sparnatural-config-datasources#SPARQLQuery"/>
        <sparnatural-config-datasources:queryString>SELECT ?uri ?count (CONCAT(STR(?theLabel), &apos; (&apos;, STR(?count), &apos;)&apos;) AS ?label) (STR(?theLabel) AS ?itemLabel)
WHERE {
  {
  SELECT ?uri ?count ?theLabel
  WHERE {
  {
    SELECT DISTINCT ?uri (COUNT(?domain) AS ?count)
    WHERE {
      ?domain $type $domain .
      ?domain $property ?uri .
      FILTER(isIRI(?uri))
    }
    GROUP BY ?uri
  }
  ?uri $labelPath ?theLabel .
  FILTER(lang(?theLabel) = &quot;&quot; || lang(?theLabel) = $lang)
  }
  ORDER BY UCASE(?theLabel)
  LIMIT 500
  }
}
ORDER BY UCASE(STR(?label))</sparnatural-config-datasources:queryString>
    </owl:NamedIndividual>
    


    <!-- http://data.sparna.fr/ontologies/sparnatural-config-datasources#query_list_label_count -->

    <owl:NamedIndividual rdf:about="http://data.sparna.fr/ontologies/sparnatural-config-datasources#query_list_label_count">
        <rdf:type rdf:resource="http://data.sparna.fr/ontologies/sparnatural-config-datasources#SPARQLQuery"/>
        <sparnatural-config-datasources:queryString>SELECT ?uri ?count (CONCAT(STR(?theLabel), &apos; (&apos;, STR(?count), &apos;)&apos;) AS ?label) (STR(?theLabel) AS ?itemLabel)
WHERE {
  {
  SELECT ?uri ?count ?theLabel
  WHERE {
  {
    SELECT DISTINCT ?uri (COUNT(?domain) AS ?count)
    WHERE {
      ?domain $type $domain .
      ?domain $property ?uri .
      FILTER(isIRI(?uri))
    }
    GROUP BY ?uri
  }
  ?uri $labelPath ?theLabel .
  FILTER(lang(?theLabel) = &quot;&quot; || lang(?theLabel) = $lang)
  }
  ORDER BY DESC(?count) UCASE(?theLabel)
  LIMIT 500
  }
}
ORDER BY DESC(?count) UCASE(STR(?label))</sparnatural-config-datasources:queryString>
    </owl:NamedIndividual>
    


    <!-- http://data.sparna.fr/ontologies/sparnatural-config-datasources#query_list_label_with_range_alpha -->

    <owl:NamedIndividual rdf:about="http://data.sparna.fr/ontologies/sparnatural-config-datasources#query_list_label_with_range_alpha">
        <rdf:type rdf:resource="http://data.sparna.fr/ontologies/sparnatural-config-datasources#SPARQLQuery"/>
        <sparnatural-config-datasources:queryString>SELECT DISTINCT ?uri ?label
WHERE {
    ?domain $type $domain .
    ?domain $property ?uri .
    # range criteria
    ?uri $type $range .
    ?uri $labelPath ?label .
    FILTER(isIRI(?uri))
    FILTER(lang(?label) = &quot;&quot; || lang(?label) = $lang)
}
ORDER BY UCASE(STR(?label))
LIMIT 500</sparnatural-config-datasources:queryString>
    </owl:NamedIndividual>
    


    <!-- http://data.sparna.fr/ontologies/sparnatural-config-datasources#query_list_label_with_range_alpha_with_count -->

    <owl:NamedIndividual rdf:about="http://data.sparna.fr/ontologies/sparnatural-config-datasources#query_list_label_with_range_alpha_with_count">
        <rdf:type rdf:resource="http://data.sparna.fr/ontologies/sparnatural-config-datasources#SPARQLQuery"/>
        <sparnatural-config-datasources:queryString>SELECT ?uri ?count (CONCAT(STR(?theLabel), &apos; (&apos;, STR(?count), &apos;)&apos;) AS ?label) (STR(?theLabel) AS ?itemLabel)
WHERE {
  {
  SELECT ?uri ?count ?theLabel
  WHERE {
  {
    SELECT DISTINCT ?uri (COUNT(?domain) AS ?count)
    WHERE {
      ?domain $type $domain .
      ?domain $property ?uri .
      FILTER(isIRI(?uri))
      # range criteria
      ?uri $type $range .
    }
    GROUP BY ?uri
  }
  ?uri $labelPath ?theLabel .
  FILTER(lang(?theLabel) = &quot;&quot; || lang(?theLabel) = $lang)
  }
  ORDER BY UCASE(?theLabel)
  LIMIT 500
  }
}
ORDER BY UCASE(STR(?label))</sparnatural-config-datasources:queryString>
    </owl:NamedIndividual>
    


    <!-- http://data.sparna.fr/ontologies/sparnatural-config-datasources#query_list_label_with_range_count -->

    <owl:NamedIndividual rdf:about="http://data.sparna.fr/ontologies/sparnatural-config-datasources#query_list_label_with_range_count">
        <rdf:type rdf:resource="http://data.sparna.fr/ontologies/sparnatural-config-datasources#SPARQLQuery"/>
        <sparnatural-config-datasources:queryString>SELECT ?uri ?count (CONCAT(STR(?theLabel), &apos; (&apos;, STR(?count), &apos;)&apos;) AS ?label) (STR(?theLabel) AS ?itemLabel)
WHERE {
  {
  SELECT ?uri ?count ?theLabel
  WHERE {
  {
    SELECT DISTINCT ?uri (COUNT(?domain) AS ?count)
    WHERE {
      ?domain $type $domain .
      ?domain $property ?uri .
      FILTER(isIRI(?uri))
      ?uri $type $range .
    }
    GROUP BY ?uri
  }
  ?uri $labelPath ?theLabel .
  FILTER(lang(?theLabel) = &quot;&quot; || lang(?theLabel) = $lang)
  }
  ORDER BY DESC(?count) UCASE(?theLabel)
  LIMIT 500
  }
}
ORDER BY DESC(?count) UCASE(STR(?label))</sparnatural-config-datasources:queryString>
    </owl:NamedIndividual>
    


    <!-- http://data.sparna.fr/ontologies/sparnatural-config-datasources#query_literal_list_alpha -->

    <owl:NamedIndividual rdf:about="http://data.sparna.fr/ontologies/sparnatural-config-datasources#query_literal_list_alpha">
        <rdf:type rdf:resource="http://data.sparna.fr/ontologies/sparnatural-config-datasources#SPARQLQuery"/>
        <sparnatural-config-datasources:queryString>SELECT DISTINCT ?value (STR(?value) AS ?label)
WHERE {
    ?domain $type $domain .
    ?domain $property ?value .
}
ORDER BY UCASE(STR(?label))
LIMIT 500</sparnatural-config-datasources:queryString>
    </owl:NamedIndividual>
    


    <!-- http://data.sparna.fr/ontologies/sparnatural-config-datasources#query_literal_list_alpha_with_count -->

    <owl:NamedIndividual rdf:about="http://data.sparna.fr/ontologies/sparnatural-config-datasources#query_literal_list_alpha_with_count">
        <rdf:type rdf:resource="http://data.sparna.fr/ontologies/sparnatural-config-datasources#SPARQLQuery"/>
        <sparnatural-config-datasources:queryString>SELECT ?count (CONCAT(STR(?theLabel), &apos; (&apos;, STR(?count), &apos;)&apos;) AS ?label) (STR(?theLabel) AS ?itemLabel)
WHERE {
  {
  SELECT DISTINCT ?count ?theLabel
  WHERE {
  {
    SELECT DISTINCT ?theLabel (COUNT(?theLabel) AS ?count)
    WHERE {
      ?domain $type $domain .
      ?domain $property ?theLabel .
      FILTER(lang(?theLabel) = &quot;&quot; || lang(?theLabel) = $lang)
    }
    GROUP BY ?theLabel
  }
  }
  ORDER BY UCASE(?theLabel)
  LIMIT 500
  }
}
ORDER BY UCASE(STR(?label))</sparnatural-config-datasources:queryString>
    </owl:NamedIndividual>
    


    <!-- http://data.sparna.fr/ontologies/sparnatural-config-datasources#query_literal_list_count -->

    <owl:NamedIndividual rdf:about="http://data.sparna.fr/ontologies/sparnatural-config-datasources#query_literal_list_count">
        <rdf:type rdf:resource="http://data.sparna.fr/ontologies/sparnatural-config-datasources#SPARQLQuery"/>
        <sparnatural-config-datasources:queryString>SELECT ?count (CONCAT(STR(?theLabel), &apos; (&apos;, STR(?count), &apos;)&apos;) AS ?label) (STR(?theLabel) AS ?itemLabel)
WHERE {
  {
  SELECT DISTINCT ?count ?theLabel
  WHERE {
  {
    SELECT DISTINCT ?theLabel (COUNT(?theLabel) AS ?count)
    WHERE {
      ?domain $type $domain .
      ?domain $property ?theLabel .
      FILTER(lang(?theLabel) = &quot;&quot; || lang(?theLabel) = $lang)
    }
    GROUP BY ?theLabel
  }
  }
  ORDER BY DESC(?count) UCASE(?theLabel)
  LIMIT 500
  }
}
ORDER BY DESC(?count) UCASE(STR(?label))</sparnatural-config-datasources:queryString>
    </owl:NamedIndividual>
    


    <!-- http://data.sparna.fr/ontologies/sparnatural-config-datasources#query_search_URI_contains -->

    <owl:NamedIndividual rdf:about="http://data.sparna.fr/ontologies/sparnatural-config-datasources#query_search_URI_contains">
        <rdf:type rdf:resource="http://data.sparna.fr/ontologies/sparnatural-config-datasources#SPARQLQuery"/>
        <sparnatural-config-datasources:queryString>SELECT DISTINCT ?uri ?label
WHERE {
  ?domain $type $domain .
  ?domain $property ?uri .
  ?uri $type $range .
  FILTER(isIRI(?uri))
  BIND(STR(?uri) AS ?label)
  FILTER(CONTAINS(LCASE(?label), LCASE(&quot;$key&quot;))) 
} 
ORDER BY UCASE(STR(?label))
LIMIT 15</sparnatural-config-datasources:queryString>
    </owl:NamedIndividual>
    


    <!-- http://data.sparna.fr/ontologies/sparnatural-config-datasources#query_search_label_bifcontains -->

    <owl:NamedIndividual rdf:about="http://data.sparna.fr/ontologies/sparnatural-config-datasources#query_search_label_bifcontains">
        <rdf:type rdf:resource="http://data.sparna.fr/ontologies/sparnatural-config-datasources#SPARQLQuery"/>
        <sparnatural-config-datasources:queryString>PREFIX bif: &lt;http://www.openlinksw.com/schemas/bif#&gt;
SELECT DISTINCT ?uri ?label
 WHERE {
  ?domain $type $domain .
  ?domain $property ?uri .
  ?uri $type $range .
  ?uri $labelPath ?label .
  FILTER(isIRI(?uri))
  FILTER(lang(?label) = &apos;&apos; || lang(?label) = $lang )
  # Note the single quote to handle space character
  ?label bif:contains &quot;&apos;$key&apos;&quot; . 
} 
ORDER BY UCASE(STR(?label))
LIMIT 15</sparnatural-config-datasources:queryString>
    </owl:NamedIndividual>
    


    <!-- http://data.sparna.fr/ontologies/sparnatural-config-datasources#query_search_label_contains -->

    <owl:NamedIndividual rdf:about="http://data.sparna.fr/ontologies/sparnatural-config-datasources#query_search_label_contains">
        <rdf:type rdf:resource="http://data.sparna.fr/ontologies/sparnatural-config-datasources#SPARQLQuery"/>
        <sparnatural-config-datasources:queryString>SELECT DISTINCT ?uri ?label
WHERE {
  ?domain $type $domain .
  ?domain $property ?uri .
  ?uri $type $range .
  ?uri $labelPath ?label .
  FILTER(isIRI(?uri))
  FILTER(lang(?label) = &apos;&apos; || lang(?label) = $lang)
  FILTER(CONTAINS(LCASE(STR(?label)), LCASE(&quot;$key&quot;))) 
  BIND( IF( STRSTARTS(LCASE(STR(?label)), LCASE(&quot;$key&quot;)),0,9 ) AS ?starts )
} 
ORDER BY UCASE(STR(?label))
LIMIT 15</sparnatural-config-datasources:queryString>
    </owl:NamedIndividual>
    


    <!-- http://data.sparna.fr/ontologies/sparnatural-config-datasources#query_search_label_strstarts -->

    <owl:NamedIndividual rdf:about="http://data.sparna.fr/ontologies/sparnatural-config-datasources#query_search_label_strstarts">
        <rdf:type rdf:resource="http://data.sparna.fr/ontologies/sparnatural-config-datasources#SPARQLQuery"/>
        <sparnatural-config-datasources:queryString>SELECT DISTINCT ?uri ?label
WHERE {
  ?domain $type $domain .
  ?domain $property ?uri .
  ?uri $type $range .
  ?uri $labelPath ?label .
  FILTER(isIRI(?uri))
  FILTER(lang(?label) = &apos;&apos; || lang(?label) = $lang)
  FILTER(STRSTARTS(LCASE(STR(?label)), LCASE(&quot;$key&quot;))) 
} 
ORDER BY UCASE(STR(?label))
LIMIT 15</sparnatural-config-datasources:queryString>
    </owl:NamedIndividual>
    


    <!-- http://data.sparna.fr/ontologies/sparnatural-config-datasources#query_search_literal_contains -->

    <owl:NamedIndividual rdf:about="http://data.sparna.fr/ontologies/sparnatural-config-datasources#query_search_literal_contains">
        <rdf:type rdf:resource="http://data.sparna.fr/ontologies/sparnatural-config-datasources#SPARQLQuery"/>
        <sparnatural-config-datasources:queryString>SELECT DISTINCT ?value ?label
WHERE {
  ?domain $type $domain .
  ?domain $property ?value .
  FILTER(isLiteral(?value))
  BIND(STR(?value) AS ?label)
  FILTER(CONTAINS(LCASE(STR(?value)), LCASE(&quot;$key&quot;))) 
} 
ORDER BY UCASE(STR(?label))
LIMIT 15</sparnatural-config-datasources:queryString>
    </owl:NamedIndividual>
    


    <!-- http://data.sparna.fr/ontologies/sparnatural-config-datasources#query_search_literal_strstarts -->

    <owl:NamedIndividual rdf:about="http://data.sparna.fr/ontologies/sparnatural-config-datasources#query_search_literal_strstarts">
        <rdf:type rdf:resource="http://data.sparna.fr/ontologies/sparnatural-config-datasources#SPARQLQuery"/>
        <sparnatural-config-datasources:queryString>SELECT DISTINCT ?value ?label
WHERE {
  ?domain $type $domain .
  ?domain $property ?value .
  FILTER(isLiteral(?value))
  BIND(STR(?value) AS ?label)
  FILTER(STRSTARTS(LCASE(STR(?value)), LCASE(&quot;$key&quot;))) 
} 
ORDER BY UCASE(STR(?label))
LIMIT 15</sparnatural-config-datasources:queryString>
    </owl:NamedIndividual>
    


    <!-- http://data.sparna.fr/ontologies/sparnatural-config-datasources#query_tree_children -->

    <owl:NamedIndividual rdf:about="http://data.sparna.fr/ontologies/sparnatural-config-datasources#query_tree_children">
        <rdf:type rdf:resource="http://data.sparna.fr/ontologies/sparnatural-config-datasources#SPARQLQuery"/>
        <sparnatural-config-datasources:queryString># Selects the children of a node
SELECT DISTINCT ?uri ?label ?hasChildren
WHERE {
  $node $childrenPath ?uri .
  ?uri $labelPath ?label .
  FILTER(isIRI(?uri))
  FILTER(lang(?label) = &apos;&apos; || lang(?label) = $lang)
  OPTIONAL {
  	?uri $childrenPath ?children .
  }
  BIND(IF(bound(?children),true,false) AS ?hasChildren)
}
ORDER BY UCASE(STR(?label))</sparnatural-config-datasources:queryString>
    </owl:NamedIndividual>
    


    <!-- http://data.sparna.fr/ontologies/sparnatural-config-datasources#query_tree_children_with_count -->

    <owl:NamedIndividual rdf:about="http://data.sparna.fr/ontologies/sparnatural-config-datasources#query_tree_children_with_count">
        <rdf:type rdf:resource="http://data.sparna.fr/ontologies/sparnatural-config-datasources#SPARQLQuery"/>
        <sparnatural-config-datasources:queryString>SELECT ?uri (CONCAT(STR(?theLabel), &apos; (&apos;, STR(?count), &apos;)&apos;) AS ?label) ?hasChildren ?count (STR(?theLabel) AS ?itemLabel)
WHERE {
  {
  SELECT DISTINCT ?uri ?theLabel ?hasChildren (COUNT(?x) AS ?count)
  WHERE {
    {
      SELECT ?uri ?theLabel ?hasChildren
      WHERE {
        $node $childrenPath ?uri .
        ?uri $labelPath ?theLabel .
        FILTER(isIRI(?uri))
        FILTER(lang(?theLabel) = &apos;&apos; || lang(?theLabel) = $lang)
        OPTIONAL {
          ?uri $childrenPath ?children .
        }
        BIND(IF(bound(?children),true,false) AS ?hasChildren)
      }
    }

    OPTIONAL {
      ?x $type $domain .
      ?x $property ?uri .
      # no range criteria
      # ?uri a $range .
    }
  }
  GROUP BY ?uri ?theLabel ?hasChildren
  }
}
ORDER BY UCASE(STR(?label))</sparnatural-config-datasources:queryString>
    </owl:NamedIndividual>
    


    <!-- http://data.sparna.fr/ontologies/sparnatural-config-datasources#query_tree_root_noparent -->

    <owl:NamedIndividual rdf:about="http://data.sparna.fr/ontologies/sparnatural-config-datasources#query_tree_root_noparent">
        <rdf:type rdf:resource="http://data.sparna.fr/ontologies/sparnatural-config-datasources#SPARQLQuery"/>
        <sparnatural-config-datasources:queryString>SELECT ?uri ?label ?hasChildren
WHERE {
  ?uri $type $range .
  FILTER NOT EXISTS {
    ?parent $childrenPath ?uri .
  }
  ?uri $labelPath ?label .
  FILTER(isIRI(?uri))
  FILTER(lang(?label) = &apos;&apos; || lang(?label) = $lang)
  OPTIONAL {
    ?uri $childrenPath ?children .
  }
  BIND(IF(bound(?children),true,false) AS ?hasChildren)
}
ORDER BY UCASE(STR(?label))</sparnatural-config-datasources:queryString>
    </owl:NamedIndividual>
    


    <!-- http://data.sparna.fr/ontologies/sparnatural-config-datasources#query_tree_root_noparent_with_count -->

    <owl:NamedIndividual rdf:about="http://data.sparna.fr/ontologies/sparnatural-config-datasources#query_tree_root_noparent_with_count">
        <rdf:type rdf:resource="http://data.sparna.fr/ontologies/sparnatural-config-datasources#SPARQLQuery"/>
        <sparnatural-config-datasources:queryString>SELECT ?uri (CONCAT(STR(?theLabel), &apos; (&apos;, STR(?count), &apos;)&apos;) AS ?label) ?hasChildren ?count (STR(?theLabel) AS ?itemLabel)
WHERE {
  {
  SELECT ?uri ?theLabel ?hasChildren (COUNT(?x) AS ?count)
  WHERE {
    {
      SELECT ?uri ?theLabel ?hasChildren
      WHERE {
        ?uri $type $range .
        FILTER NOT EXISTS {
          ?parent $childrenPath ?uri .
        }
        ?uri $labelPath ?theLabel .
        FILTER(isIRI(?uri))
        FILTER(lang(?theLabel) = &apos;&apos; || lang(?theLabel) = $lang)
        OPTIONAL {
          ?uri $childrenPath ?children .
        }
        BIND(IF(bound(?children),true,false) AS ?hasChildren)
      }
    }

    OPTIONAL {
      ?x $type $domain .
      ?x $property ?uri .
    }
  }
  GROUP BY ?uri ?theLabel ?hasChildren
  }
} 
ORDER BY UCASE(STR(?label))</sparnatural-config-datasources:queryString>
    </owl:NamedIndividual>
    


    <!-- http://data.sparna.fr/ontologies/sparnatural-config-datasources#search_URI_contains -->

    <owl:NamedIndividual rdf:about="http://data.sparna.fr/ontologies/sparnatural-config-datasources#search_URI_contains">
        <rdf:type rdf:resource="http://data.sparna.fr/ontologies/sparnatural-config-datasources#SparqlSearchDatasource"/>
        <sparnatural-config-datasources:queryTemplate rdf:resource="http://data.sparna.fr/ontologies/sparnatural-config-datasources#query_search_URI_contains"/>
        <rdfs:comment xml:lang="en">Searches for entities by looking up the provided $key in their URI string using the CONTAINS SPARQL function.</rdfs:comment>
    </owl:NamedIndividual>
    


    <!-- http://data.sparna.fr/ontologies/sparnatural-config-datasources#search_dctermstitle_bifcontains -->

    <owl:NamedIndividual rdf:about="http://data.sparna.fr/ontologies/sparnatural-config-datasources#search_dctermstitle_bifcontains">
        <rdf:type rdf:resource="http://data.sparna.fr/ontologies/sparnatural-config-datasources#SparqlSearchDatasource"/>
        <sparnatural-config-datasources:queryTemplate rdf:resource="http://data.sparna.fr/ontologies/sparnatural-config-datasources#query_search_label_bifcontains"/>
        <sparnatural-config-datasources:labelProperty rdf:resource="http://purl.org/dc/terms/title"/>
        <rdfs:comment xml:lang="en">Searches for entities by looking up the provided $key inside their dcterms:title using the bif:contains Virtuoso function.</rdfs:comment>
    </owl:NamedIndividual>
    


    <!-- http://data.sparna.fr/ontologies/sparnatural-config-datasources#search_dctermstitle_contains -->

    <owl:NamedIndividual rdf:about="http://data.sparna.fr/ontologies/sparnatural-config-datasources#search_dctermstitle_contains">
        <rdf:type rdf:resource="http://data.sparna.fr/ontologies/sparnatural-config-datasources#SparqlSearchDatasource"/>
        <sparnatural-config-datasources:queryTemplate rdf:resource="http://data.sparna.fr/ontologies/sparnatural-config-datasources#query_search_label_contains"/>
        <sparnatural-config-datasources:labelProperty rdf:resource="http://purl.org/dc/terms/title"/>
        <rdfs:comment xml:lang="en">Searches for entities by looking up the provided $key inside their dcterms:title using the CONTAINS SPARQL function.</rdfs:comment>
    </owl:NamedIndividual>
    


    <!-- http://data.sparna.fr/ontologies/sparnatural-config-datasources#search_dctermstitle_strstarts -->

    <owl:NamedIndividual rdf:about="http://data.sparna.fr/ontologies/sparnatural-config-datasources#search_dctermstitle_strstarts">
        <rdf:type rdf:resource="http://data.sparna.fr/ontologies/sparnatural-config-datasources#SparqlSearchDatasource"/>
        <sparnatural-config-datasources:queryTemplate rdf:resource="http://data.sparna.fr/ontologies/sparnatural-config-datasources#query_search_label_strstarts"/>
        <sparnatural-config-datasources:labelProperty rdf:resource="http://purl.org/dc/terms/title"/>
        <rdfs:comment xml:lang="en">Searches for entities by looking up the provided $key at the beginning of their dcterms;title using the STRSTARTS SPARQL function.</rdfs:comment>
    </owl:NamedIndividual>
    


    <!-- http://data.sparna.fr/ontologies/sparnatural-config-datasources#search_foafname_bifcontains -->

    <owl:NamedIndividual rdf:about="http://data.sparna.fr/ontologies/sparnatural-config-datasources#search_foafname_bifcontains">
        <rdf:type rdf:resource="http://data.sparna.fr/ontologies/sparnatural-config-datasources#SparqlSearchDatasource"/>
        <sparnatural-config-datasources:queryTemplate rdf:resource="http://data.sparna.fr/ontologies/sparnatural-config-datasources#query_search_label_bifcontains"/>
        <sparnatural-config-datasources:labelProperty rdf:resource="http://xmlns.com/foaf/0.1/name"/>
        <rdfs:comment xml:lang="en">Searches for entities by looking up the provided $key inside their foaf:name using the bif:contains Virtuoso function.</rdfs:comment>
    </owl:NamedIndividual>
    


    <!-- http://data.sparna.fr/ontologies/sparnatural-config-datasources#search_foafname_contains -->

    <owl:NamedIndividual rdf:about="http://data.sparna.fr/ontologies/sparnatural-config-datasources#search_foafname_contains">
        <rdf:type rdf:resource="http://data.sparna.fr/ontologies/sparnatural-config-datasources#SparqlSearchDatasource"/>
        <sparnatural-config-datasources:queryTemplate rdf:resource="http://data.sparna.fr/ontologies/sparnatural-config-datasources#query_search_label_contains"/>
        <sparnatural-config-datasources:labelProperty rdf:resource="http://xmlns.com/foaf/0.1/name"/>
        <rdfs:comment xml:lang="en">Searches for entities by looking up the provided $key inside their foaf:name using the CONTAINS SPARQL function.</rdfs:comment>
    </owl:NamedIndividual>
    


    <!-- http://data.sparna.fr/ontologies/sparnatural-config-datasources#search_foafname_strstarts -->

    <owl:NamedIndividual rdf:about="http://data.sparna.fr/ontologies/sparnatural-config-datasources#search_foafname_strstarts">
        <rdf:type rdf:resource="http://data.sparna.fr/ontologies/sparnatural-config-datasources#SparqlSearchDatasource"/>
        <sparnatural-config-datasources:queryTemplate rdf:resource="http://data.sparna.fr/ontologies/sparnatural-config-datasources#query_search_label_strstarts"/>
        <sparnatural-config-datasources:labelProperty rdf:resource="http://xmlns.com/foaf/0.1/name"/>
        <rdfs:comment xml:lang="en">Searches for entities by looking up the provided $key at the beginning of their foaf:name using the STRSTARTS SPARQL function.</rdfs:comment>
    </owl:NamedIndividual>
    


    <!-- http://data.sparna.fr/ontologies/sparnatural-config-datasources#search_literal_contains -->

    <owl:NamedIndividual rdf:about="http://data.sparna.fr/ontologies/sparnatural-config-datasources#search_literal_contains">
        <rdf:type rdf:resource="http://data.sparna.fr/ontologies/sparnatural-config-datasources#SparqlSearchDatasource"/>
        <sparnatural-config-datasources:queryTemplate rdf:resource="http://data.sparna.fr/ontologies/sparnatural-config-datasources#query_search_literal_contains"/>
    </owl:NamedIndividual>
    


    <!-- http://data.sparna.fr/ontologies/sparnatural-config-datasources#search_literal_strstarts -->

    <owl:NamedIndividual rdf:about="http://data.sparna.fr/ontologies/sparnatural-config-datasources#search_literal_strstarts">
        <rdf:type rdf:resource="http://data.sparna.fr/ontologies/sparnatural-config-datasources#SparqlSearchDatasource"/>
        <sparnatural-config-datasources:queryTemplate rdf:resource="http://data.sparna.fr/ontologies/sparnatural-config-datasources#query_search_literal_strstarts"/>
    </owl:NamedIndividual>
    


    <!-- http://data.sparna.fr/ontologies/sparnatural-config-datasources#search_rdfslabel_bifcontains -->

    <owl:NamedIndividual rdf:about="http://data.sparna.fr/ontologies/sparnatural-config-datasources#search_rdfslabel_bifcontains">
        <rdf:type rdf:resource="http://data.sparna.fr/ontologies/sparnatural-config-datasources#SparqlSearchDatasource"/>
        <sparnatural-config-datasources:queryTemplate rdf:resource="http://data.sparna.fr/ontologies/sparnatural-config-datasources#query_search_label_bifcontains"/>
        <sparnatural-config-datasources:labelProperty rdf:resource="http://www.w3.org/2000/01/rdf-schema#label"/>
        <rdfs:comment xml:lang="en">Searches for entities by looking up the provided $key inside their rdfs:label using the bif:contains Virtuoso function.</rdfs:comment>
    </owl:NamedIndividual>
    


    <!-- http://data.sparna.fr/ontologies/sparnatural-config-datasources#search_rdfslabel_contains -->

    <owl:NamedIndividual rdf:about="http://data.sparna.fr/ontologies/sparnatural-config-datasources#search_rdfslabel_contains">
        <rdf:type rdf:resource="http://data.sparna.fr/ontologies/sparnatural-config-datasources#SparqlSearchDatasource"/>
        <sparnatural-config-datasources:queryTemplate rdf:resource="http://data.sparna.fr/ontologies/sparnatural-config-datasources#query_search_label_contains"/>
        <sparnatural-config-datasources:labelProperty rdf:resource="http://www.w3.org/2000/01/rdf-schema#label"/>
        <rdfs:comment xml:lang="en">Searches for entities by looking up the provided $key inside their rdfs:label using the CONTAINS SPARQL function.</rdfs:comment>
    </owl:NamedIndividual>
    


    <!-- http://data.sparna.fr/ontologies/sparnatural-config-datasources#search_rdfslabel_strstarts -->

    <owl:NamedIndividual rdf:about="http://data.sparna.fr/ontologies/sparnatural-config-datasources#search_rdfslabel_strstarts">
        <rdf:type rdf:resource="http://data.sparna.fr/ontologies/sparnatural-config-datasources#SparqlSearchDatasource"/>
        <sparnatural-config-datasources:queryTemplate rdf:resource="http://data.sparna.fr/ontologies/sparnatural-config-datasources#query_search_label_strstarts"/>
        <sparnatural-config-datasources:labelProperty rdf:resource="http://www.w3.org/2000/01/rdf-schema#label"/>
        <rdfs:comment xml:lang="en">Searches for entities by looking up the provided $key at the beginning of their rdfs:label using the STRSTARTS SPARQL function.</rdfs:comment>
    </owl:NamedIndividual>
    


    <!-- http://data.sparna.fr/ontologies/sparnatural-config-datasources#search_schemaname_bifcontains -->

    <owl:NamedIndividual rdf:about="http://data.sparna.fr/ontologies/sparnatural-config-datasources#search_schemaname_bifcontains">
        <rdf:type rdf:resource="http://data.sparna.fr/ontologies/sparnatural-config-datasources#SparqlSearchDatasource"/>
        <sparnatural-config-datasources:queryTemplate rdf:resource="http://data.sparna.fr/ontologies/sparnatural-config-datasources#query_search_label_bifcontains"/>
        <sparnatural-config-datasources:labelPath rdf:resource="http://schema.org/name"/>
        <rdfs:comment xml:lang="en">Searches for entities by looking up the provided $key inside their schema:name using the bif:contains Virtuoso function.</rdfs:comment>
    </owl:NamedIndividual>
    


    <!-- http://data.sparna.fr/ontologies/sparnatural-config-datasources#search_schemaname_contains -->

    <owl:NamedIndividual rdf:about="http://data.sparna.fr/ontologies/sparnatural-config-datasources#search_schemaname_contains">
        <rdf:type rdf:resource="http://data.sparna.fr/ontologies/sparnatural-config-datasources#SparqlSearchDatasource"/>
        <sparnatural-config-datasources:queryTemplate rdf:resource="http://data.sparna.fr/ontologies/sparnatural-config-datasources#query_search_label_contains"/>
        <sparnatural-config-datasources:labelProperty rdf:resource="http://schema.org/name"/>
        <rdfs:comment xml:lang="en">Searches for entities by looking up the provided $key inside their schema:name using the CONTAINS SPARQL function.</rdfs:comment>
    </owl:NamedIndividual>
    


    <!-- http://data.sparna.fr/ontologies/sparnatural-config-datasources#search_schemaname_strstarts -->

    <owl:NamedIndividual rdf:about="http://data.sparna.fr/ontologies/sparnatural-config-datasources#search_schemaname_strstarts">
        <rdf:type rdf:resource="http://data.sparna.fr/ontologies/sparnatural-config-datasources#SparqlSearchDatasource"/>
        <sparnatural-config-datasources:queryTemplate rdf:resource="http://data.sparna.fr/ontologies/sparnatural-config-datasources#query_search_label_strstarts"/>
        <sparnatural-config-datasources:labelProperty rdf:resource="http://schema.org/name"/>
        <rdfs:comment xml:lang="en">Searches for entities by looking up the provided $key at the beginning of their schema:name using the STRSTARTS SPARQL function.</rdfs:comment>
    </owl:NamedIndividual>
    


    <!-- http://data.sparna.fr/ontologies/sparnatural-config-datasources#search_skospreflabel_bifcontains -->

    <owl:NamedIndividual rdf:about="http://data.sparna.fr/ontologies/sparnatural-config-datasources#search_skospreflabel_bifcontains">
        <rdf:type rdf:resource="http://data.sparna.fr/ontologies/sparnatural-config-datasources#SparqlSearchDatasource"/>
        <sparnatural-config-datasources:queryTemplate rdf:resource="http://data.sparna.fr/ontologies/sparnatural-config-datasources#query_search_label_bifcontains"/>
        <sparnatural-config-datasources:labelPath rdf:resource="http://www.w3.org/2004/02/skos/core#prefLabel"/>
        <rdfs:comment xml:lang="en">Searches for entities by looking up the provided $key inside their skos:prefLabel using the bif:contains Virtuoso function.</rdfs:comment>
    </owl:NamedIndividual>
    


    <!-- http://data.sparna.fr/ontologies/sparnatural-config-datasources#search_skospreflabel_contains -->

    <owl:NamedIndividual rdf:about="http://data.sparna.fr/ontologies/sparnatural-config-datasources#search_skospreflabel_contains">
        <rdf:type rdf:resource="http://data.sparna.fr/ontologies/sparnatural-config-datasources#SparqlSearchDatasource"/>
        <sparnatural-config-datasources:queryTemplate rdf:resource="http://data.sparna.fr/ontologies/sparnatural-config-datasources#query_search_label_contains"/>
        <sparnatural-config-datasources:labelProperty rdf:resource="http://www.w3.org/2004/02/skos/core#prefLabel"/>
        <rdfs:comment xml:lang="en">Searches for entities by looking up the provided $key inside their skos:prefLabel using the CONTAINS SPARQL function.</rdfs:comment>
    </owl:NamedIndividual>
    


    <!-- http://data.sparna.fr/ontologies/sparnatural-config-datasources#search_skospreflabel_strstarts -->

    <owl:NamedIndividual rdf:about="http://data.sparna.fr/ontologies/sparnatural-config-datasources#search_skospreflabel_strstarts">
        <rdf:type rdf:resource="http://data.sparna.fr/ontologies/sparnatural-config-datasources#SparqlSearchDatasource"/>
        <sparnatural-config-datasources:queryTemplate rdf:resource="http://data.sparna.fr/ontologies/sparnatural-config-datasources#query_search_label_strstarts"/>
        <sparnatural-config-datasources:labelProperty rdf:resource="http://www.w3.org/2004/02/skos/core#prefLabel"/>
        <rdfs:comment xml:lang="en">Searches for entities by looking up the provided $key at the beginning of their skos:prefLabel using the STRSTARTS SPARQL function.</rdfs:comment>
    </owl:NamedIndividual>
    


    <!-- http://data.sparna.fr/ontologies/sparnatural-config-datasources#tree_children_skosnarrower -->

    <owl:NamedIndividual rdf:about="http://data.sparna.fr/ontologies/sparnatural-config-datasources#tree_children_skosnarrower">
        <rdf:type rdf:resource="http://data.sparna.fr/ontologies/sparnatural-config-datasources#SparqlTreeChildrenDatasource"/>
        <sparnatural-config-datasources:queryTemplate rdf:resource="http://data.sparna.fr/ontologies/sparnatural-config-datasources#query_tree_children"/>
        <sparnatural-config-datasources:childrenPath>&lt;http://www.w3.org/2004/02/skos/core#narrower&gt;|^&lt;http://www.w3.org/2004/02/skos/core#broader&gt;</sparnatural-config-datasources:childrenPath>
        <sparnatural-config-datasources:labelPath>&lt;http://www.w3.org/2004/02/skos/core#prefLabel&gt;</sparnatural-config-datasources:labelPath>
    </owl:NamedIndividual>
    


    <!-- http://data.sparna.fr/ontologies/sparnatural-config-datasources#tree_children_skosnarrower_with_count -->

    <owl:NamedIndividual rdf:about="http://data.sparna.fr/ontologies/sparnatural-config-datasources#tree_children_skosnarrower_with_count">
        <rdf:type rdf:resource="http://data.sparna.fr/ontologies/sparnatural-config-datasources#SparqlTreeChildrenDatasource"/>
        <sparnatural-config-datasources:queryTemplate rdf:resource="http://data.sparna.fr/ontologies/sparnatural-config-datasources#query_tree_children_with_count"/>
        <sparnatural-config-datasources:childrenPath>&lt;http://www.w3.org/2004/02/skos/core#narrower&gt;|^&lt;http://www.w3.org/2004/02/skos/core#broader&gt;</sparnatural-config-datasources:childrenPath>
        <sparnatural-config-datasources:labelPath>&lt;http://www.w3.org/2004/02/skos/core#prefLabel&gt;</sparnatural-config-datasources:labelPath>
    </owl:NamedIndividual>
    


    <!-- http://data.sparna.fr/ontologies/sparnatural-config-datasources#tree_root_skostopconcept -->

    <owl:NamedIndividual rdf:about="http://data.sparna.fr/ontologies/sparnatural-config-datasources#tree_root_skostopconcept">
        <rdf:type rdf:resource="http://data.sparna.fr/ontologies/sparnatural-config-datasources#SparqlTreeRootDatasource"/>
        <sparnatural-config-datasources:queryString>PREFIX skos: &lt;http://www.w3.org/2004/02/skos/core#&gt;
SELECT DISTINCT ?uri ?label ?hasChildren
WHERE {
  $range skos:hasTopConcept|^skos:topConceptOf ?uri .
  ?uri skos:prefLabel ?label .
  FILTER(isIRI(?uri))
  FILTER(lang(?label) = &apos;&apos; || lang(?label) = $lang)
  OPTIONAL {
    ?uri skos:narrower|^skos:broader ?children .
  }
  BIND(IF(bound(?children),true,false) AS ?hasChildren)
}
ORDER BY UCASE(STR(?label))</sparnatural-config-datasources:queryString>
    </owl:NamedIndividual>
    


    <!-- http://data.sparna.fr/ontologies/sparnatural-config-datasources#tree_root_skostopconcept_with_count -->

    <owl:NamedIndividual rdf:about="http://data.sparna.fr/ontologies/sparnatural-config-datasources#tree_root_skostopconcept_with_count">
        <rdf:type rdf:resource="http://data.sparna.fr/ontologies/sparnatural-config-datasources#SparqlTreeRootDatasource"/>
        <sparnatural-config-datasources:queryString>PREFIX skos: &lt;http://www.w3.org/2004/02/skos/core#&gt;
SELECT ?uri (CONCAT(STR(?theLabel), &apos; (&apos;, STR(?count), &apos;)&apos;) AS ?label) ?hasChildren ?count
WHERE {
  {
    SELECT ?uri ?theLabel ?hasChildren (COUNT(?x) AS ?count)
    WHERE {
      {
        SELECT ?uri ?theLabel ?hasChildren
        WHERE {
          $range skos:hasTopConcept|^skos:topConceptOf ?uri .
          ?uri skos:prefLabel ?theLabel .
          FILTER(isIRI(?uri))
          FILTER(lang(?theLabel) = &apos;&apos; || lang(?theLabel) = $lang)
          OPTIONAL {
            ?uri skos:narrower|^skos:broader ?children .
          }
          BIND(IF(bound(?children),true,false) AS ?hasChildren)
        }
      }

      OPTIONAL {
        ?x a $domain .
        ?x $property ?uri .
        # no range criteria
        # ?uri a $range .
      }
    }
    GROUP BY ?uri ?theLabel ?hasChildren
  }
} ORDER BY UCASE(STR(?label))</sparnatural-config-datasources:queryString>
    </owl:NamedIndividual>
    


    <!-- http://data.sparna.fr/ontologies/sparnatural-config-datasources/query_tree_root_domain -->

    <owl:NamedIndividual rdf:about="http://data.sparna.fr/ontologies/sparnatural-config-datasources/query_tree_root_domain">
        <rdf:type rdf:resource="http://data.sparna.fr/ontologies/sparnatural-config-datasources#SPARQLQuery"/>
        <sparnatural-config-datasources:queryString>PREFIX rdfs: &lt;http://www.w3.org/2000/01/rdf-schema#&gt;
SELECT DISTINCT ?uri ?label ?hasChildren
WHERE {
  VALUES ?uri {$domain}
  ?uri $labelPath ?label .
  OPTIONAL {
    ?uri $childrenPath ?children .
  }
  FILTER(lang(?label) = &apos;&apos; || lang(?label) = $lang)
  BIND(IF(bound(?children),true,false) AS ?hasChildren)
}</sparnatural-config-datasources:queryString>
        <rdfs:comment xml:lang="en">Assumes that the domain URI is the root of the tree we want to build. Useful to build hierarchies based on rdfs:subClassOf.</rdfs:comment>
    </owl:NamedIndividual>
    


    <!-- http://data.sparna.fr/ontologies/sparnatural-config-datasources/tree_children_subClassOf -->

    <owl:NamedIndividual rdf:about="http://data.sparna.fr/ontologies/sparnatural-config-datasources/tree_children_subClassOf">
        <rdf:type rdf:resource="http://data.sparna.fr/ontologies/sparnatural-config-datasources#SparqlTreeChildrenDatasource"/>
        <sparnatural-config-datasources:queryTemplate rdf:resource="http://data.sparna.fr/ontologies/sparnatural-config-datasources#query_tree_children"/>
        <sparnatural-config-datasources:childrenPath>^&lt;http://www.w3.org/2000/01/rdf-schema#subClassOf&gt;</sparnatural-config-datasources:childrenPath>
        <sparnatural-config-datasources:labelPath>&lt;http://www.w3.org/2000/01/rdf-schema#label&gt;</sparnatural-config-datasources:labelPath>
    </owl:NamedIndividual>
    


    <!-- http://data.sparna.fr/ontologies/sparnatural-config-datasources/tree_root_domain_subClassOf -->

    <owl:NamedIndividual rdf:about="http://data.sparna.fr/ontologies/sparnatural-config-datasources/tree_root_domain_subClassOf">
        <rdf:type rdf:resource="http://data.sparna.fr/ontologies/sparnatural-config-datasources#SparqlTreeRootDatasource"/>
        <sparnatural-config-datasources:queryTemplate rdf:resource="http://data.sparna.fr/ontologies/sparnatural-config-datasources/query_tree_root_domain"/>
        <sparnatural-config-datasources:childrenPath>^&lt;http://www.w3.org/2000/01/rdf-schema#subClassOf&gt;</sparnatural-config-datasources:childrenPath>
        <sparnatural-config-datasources:labelPath>&lt;http://www.w3.org/2000/01/rdf-schema#label&gt;</sparnatural-config-datasources:labelPath>
    </owl:NamedIndividual>
</rdf:RDF>



<!-- Generated by the OWL API (version 4.5.29.2024-05-13T12:11:03Z) https://github.com/owlcs/owlapi -->

